\documentclass[english,a4]{article}

\usepackage{amsmath,amsthm,amssymb}
\usepackage{enumitem}
\usepackage{tikz,tikz-cd}
\usepackage{microtype}
\usepackage[mathscr]{euscript}
\usepackage{mathtools}
\usepackage{hyperref}
\usepackage[capitalize]{cleveref}

\input macros%
\input macros2%

\hypersetup{
    colorlinks,
    linkcolor={red!50!black},
    citecolor={blue!50!black},
    urlcolor={blue!80!black}
}

\setlist[enumerate]{label=(\roman*)}

\title{{On symmetries of spheres in univalent foundations}}%
\author{Pierre Cagne\thanks{Universitetet i Bergen} \and Nicolai
  Kraus\thanks{University of Birmingham} \and Marc
  Bezem\thanks{Universitetet i Bergen}}%

\date{\normalsize Last updated on \today}%

%% global tikz styles
\tikzset{cell/.style={%
    shorten <=1em,%
    shorten >=1em,
    /tikz/commutative diagrams/Rightarrow
  }%
}%

\renewcommand{\ap}[1]{\left[{#1}\right]}

\begin{document}

\maketitle

\begin{abstract}
  In this paper, we investigate the symmetries of the spheres $\Sn n$
  ($n\geq 1)$ in univalent foundations.

  The case $n=1$ has a slick answer: $(\Sc = \Sc) \weq (\Sc +
  \Sc)$. Unfortunately, it is expected that the result does not
  generalize for $n>1$. However, we show that the type $\Sn n = \Sn n$
  has two equivalent connected components and we exhibit members for
  each component.
\end{abstract}


\section{Introduction}

In this paper, we are interested in the description of the type
$\Sn n = \Sn n$ ($n\geq 1$) where $\Sn n$ is the $n$-dimensional
sphere, as defined in the HoTT-book (cf.~\cite{HoTT}).

To be fully precise and to fix notations, we work inside an
intuitionistic Martin-LÃ¶f's type theory with $\Sigma$-, $\Pi$- and
$\mathrm{Id}$-types and with a cumulative hierarchy of universes,
simply written $\UU$, for which Voevodsky's univalence axiom hold. The
transport along $p$ in a type family $T:A\to \UU$ is denoted
$\trp [T] p$, and $\pathover u T p v$ denotes $\trp [T] p {(u)} = v$.
For any dependent function $f\from\prod_{x\from A}T(x)$,
the function
\begin{displaymath}
  \ap f:\prod_{x,y\from A}\prod_{p\from x=y} \pathover {f(x)} T p
  {f(y)}
\end{displaymath}
denotes the dependent application of $f$. We usually leave out the two
first arguments of $\ap f$ as they are inferable, and we write simply
$\ap f (p)$ for a path $p:x=y$. As in \cite{HoTT}, we call a type $A$
a {\em proposition} if the type $\prod_{x,y\from A} x=y$ contains an
element.

We postulate a type $\NN$ of natural numbers and a type $\ZZ$ of
integers with their respective inductive properties
(cf.~\cite[Ch.??]{HoTT}). We allow also several higher inductive types
that are defined in the HoTT-book: propositional truncation,
suspension, and the circle. Considering their importance in this
paper, we recall them in full\footnote{\color{red}Or maybe we should
  make an appendix of that? MB is for an appendix!}:
\begin{enumerate}
\item the {\em propositional truncation} of a type $A$ is a type
  $\Trunc A$ defined by
  \begin{itemize}
  \item a map $\trunc \blank \from A \to \Trunc A$, and
  \item a dependent function
    $\istrunc {-1} \from \prod_{x,y\from \Trunc A} x=y$
  \end{itemize}
  with the following induction rule:
  \begin{quote}
    given a type family $T\from \Trunc A \to \UU$ such that every
    $T(x)$ is a proposition for each $x\from \Trunc A$, every
    dependent function
    \begin{displaymath}
      s\from \prod_{a\from A}T(\trunc a)
    \end{displaymath}
    defines a dependent function
    \begin{displaymath}
      \ind(s)\from\prod_{x\from \Trunc A} T(x)
    \end{displaymath}
    such that $\ind(s)(\trunc a) \jdeq s(a)$ for all $a\from A$.
  \end{quote}
\item the {\em suspension} of a type $A$ is a type $\susp A$ defined
  by
  \begin{itemize}
  \item two elements $N,S\from \susp A$, and
  \item a  map $\mrd \from A \to (N=S)$
  \end{itemize}
  with the following induction rule:
  \begin{quote}
    given a type family $T\from \susp A \to \UU$, every dependent
    triple of elements
    \begin{displaymath}
      n\from T(N), \quad s\from T(S),\quad
      m\from \prod_{a\from A}\pathover n T {\mrd a} s
    \end{displaymath}
    defines a dependent function
    \begin{displaymath}
      \ind(n,s,m)\from\prod_{x\from \susp A} T(x)
    \end{displaymath}
    such that
    \begin{gather*}
      \ind(n,s,m)(N) \jdeq n,\quad \ind(n,s,m)(S) \jdeq s,\\
      \ap{\ind(n,s,m)}(\mrd a) = m(a)\ \text{for all}\ a\from A.
    \end{gather*}
  \end{quote}
\item the {\em circle} $\Sc$ is a type defined by
  \begin{itemize}
  \item an element $\base \from \Sc$, and
  \item a path $\Sloop: \base = \base$
  \end{itemize}
  with the following induction rule:
  \begin{quote}
    given a type family $T\from \Sc \to \UU$, every dependent pair of
    elements
    \begin{displaymath}
      b\from T(\base), \quad \ell\from \pathover b T \Sloop b
    \end{displaymath}
    defines a dependent function
    \begin{displaymath}
      \ind(b,\ell)\from\prod_{x\from \Sc} T(x)
    \end{displaymath}
    such that
    \begin{displaymath}
      \ind(b,\ell)(\base) \jdeq b,\quad \ap{\ind(b,\ell)}(\Sloop) = \ell \,.
    \end{displaymath}
  \end{quote}
\end{enumerate}
The spheres $\Sn n$ are then defined by induction on $n:\NN$ by
$\Sn n \defequi \susp {(\Sn {n-1})}$ for all $n\geq 1$.

\paragraph{Plan of the paper.}%
In \cref{sec:circle-case}, we show carefully that the type $\Sc = \Sc$
is equivalent to $\Sc + \Sc$. Maybe surprising at first, this result
is quite straightforward once we unravel the details.

In \cref{sec:sphere}, we deal with the case $n=2$. Because the
equivalence of the case $n=1$ relies heavily on $\Omega(\Sc)\weq \ZZ$
being an abelian group, we can not expect to generalize the proof for
$n=2$. However, a careful analysis of Brunerie's proof of
$\pi_2(\Sp) \weq \ZZ$ allows us to prove that the type $\Sp=\Sp$ has
exactly two connected components, equivalent to one another. 
Determining a type with a simple description that is
equivalent to these components is a challenge in itself, still open,
to the authors' knowledge.

In \cref{sec:higher-sphere}, we propagate the result by induction on
$n\geq 2$: the type $\Sn n = \Sn n$ has exactly two connected
components, equivalent to one another. Each induction step relies on
Freudenthal's suspension theorem.

\section{Symmetries of the circle}
\label{sec:circle-case}%

In this section, we will provide an equivalence:
\begin{equation}
  \label{eq:symm-cricle}%
  (\Sc = \Sc) \weq \Sc+\Sc.
\end{equation}
We will treat univalence as transparent, so that equivalences
$f:\Sc\weq \Sc$ will be treated as elements of $\Sc=\Sc$ without any
warning. In particular, we shall write as if
``$\refl \Sc \jdeq \id_\Sc$''.

To provide an equivalence of type \cref{eq:symm-cricle}, we proceed
in several steps:
\begin{itemize}
\item first, we will describe two elements of $\Sc=\Sc$;
\item next, we will prove that these two elements are not equal (and
hence in different connected components);
\item then, we will prove that every equivalence in $\Sc=\Sc$ is
  merely equal to one of these two elements;
\item finally, we will conclude by exhibiting an equivalence between
  $\Sc$ and the connected component of each of these two elements.
\end{itemize}

The first element is simply the identity equivalence $\id_\Sc$. The
second element is the function
$-\id_\Sc \defequi \ind(\base,\inv{\Sloop})$ defined by
$\Sc$-induction in the constant type family at $\Sc$. In other words,
$-\id_\Sc$ is the (propositionally) unique function $\Sc \to \Sc$ such
that:
\begin{displaymath}
  -\id_\Sc(\base) \jdeq \base%
  \quad\text{and}\quad%
  \ap{-\id_\Sc}(\Sloop) = \inv{\Sloop}.
\end{displaymath}
Let us note that $-\id_\Sc$ is an equivalence. Indeed,
\begin{displaymath}
  -\id_\Sc \circ -\id_\Sc (\base) \jdeq \base%
  \quad\text{and}\quad%
  \ap{-\id_\Sc \circ -\id_\Sc} (\Sloop) = \inv{\left(\inv \Sloop\right)} = \Sloop.
\end{displaymath}
By $\Sc$-induction, there is only one such function, the identity
function, hence it provides a path $-\id_\Sc \circ -\id_\Sc
=\id_\Sc$. This proves that $-\id_\Sc$ is its own pseudo-inverse,
hence this is an equivalence.

\begin{lemma}
  \label{lemma:S1-id-neq-minusid}%
  The proposition $\id_\Sc \neq -\id_\Sc$ holds.
\end{lemma}
\begin{proof}
  Suppose a path $p\from\id_\Sc = -\id_\Sc$ and derive a
  contradiction. Through function extensionality, and because
  $\id_\Sc(\base) \jdeq \base \jdeq -\id_\Sc(\base)$, one gets a path
  $p(\base) \from \base = \base$, and a $2$-path
  $\ap p (\Sloop) \from \pathover \base T \Sloop \base$ where
  $T(x)\defequi (\id_\Sc(x) = -\id_\Sc(x))$ for all $x:\Sc$. One can
  easily find by induction on $q\from x=y$ a path of type
  \begin{displaymath}
    \trp [T] q (\blank) = \ap{-\id_\Sc}(q) \blank \inv{\ap{\id_\Sc}(q)}.
  \end{displaymath}
  In particular, $\ap p (\Sloop)$ provides a path of type
  $\inv\Sloop p(\base) \inv\Sloop = p(\base)$. Now recall that
  the function
  \begin{equation}
    \label{eq:loopspace-circle-Z}%
    \ZZ\to(\base=\base),\quad k \mapsto \Sloop^k 
  \end{equation}
  is an equivalence. In particular, it shows that path-composition in
  $\base=\base$ is commutative, and $\ap p (\Sloop)$ together with
  path algebra provide then a path of type $\Sloop = \inv\Sloop$. This
  is a contradiction, as it would yield a path of type $1=-1$ in $\ZZ$
  through the equivalence of \cref{eq:loopspace-circle-Z}.
\end{proof}
\cref{lemma:S1-id-neq-minusid} proves that $\id_\Sc$ and $-\id_\Sc$
lie in different connected component of $\Sc=\Sc$. We will now prove
that there are no more connected components in $\Sc=\Sc$. We will need
the following consequence of \cref{lemma:S1-id-neq-minusid}.
\begin{corollary}%
  \label{cor:S1-eq-either-isaprop}%
  For every equivalence $\varphi\from \Sc=\Sc$, the following type is
  a proposition:
  \begin{equation}
    \label{eq:S1-def-target-eq}%
    P(\varphi) \defequi \Trunc{\varphi = \id_\Sc} + \Trunc{\varphi = -\id_\Sc}.
  \end{equation}
\end{corollary}
\begin{proof}
  The type $P(\varphi)$ is the disjoint sum of two propositions. In
  order to be a proposition, it is enough (and in fact necessary) for
  the two summands to not overlap. More precisely, we need to show
  that the premise
  $\Trunc{\varphi = \id_\Sc}\times\Trunc{\varphi = -\id_\Sc}$ leads to
  absurdity. Absurdity is a proposition, so we can as well suppose the
  premise ${(\varphi = \id_\Sc)}\times{(\varphi = -\id_\Sc)}$. By
  composition of paths, it gives a path of type $\id_\Sc = -\id_\Sc$
  and \cref{lemma:S1-id-neq-minusid} allows us to derive a
  contradiction.
\end{proof}

\begin{proposition}
  \label{prop:S1-eq-either}%
  For every equivalence $\varphi\from\Sc=\Sc$, the proposition
  $P(\varphi)$ of \cref{eq:S1-def-target-eq} holds.
\end{proposition}
\begin{proof}
  Let $\varphi$ be a symmetry of the circle, and let $\psi$ denote a
  pseudo-inverse of $\varphi$. The type $\Sc$ being connected, one
  have $\Trunc{\base=\varphi(\base)}$ and
  $\Trunc{\base=\psi(\base)}$. Because the goal $P(\varphi)$ is
  propositional, one can instead suppose actual paths
  $\varphi_0\from\base=\varphi(\base)$ and
  $\psi_0\from\base=\psi(\base)$. In other words, we can suppose that
  $\varphi$ and its pseudo-inverse $\psi$ are pointed maps. Denote
  $\pi$ for a path of type $\id_\Sc=\varphi\psi$. Then one can craft a
  path of type
  $(\varphi,\varphi)_0 \circ (\psi,\psi_0) =
  (\id_\Sc,\pi_{\base}\varphi(\psi_0)\varphi_0)$. Now, consider the
  induced applications
  \begin{displaymath}
    \loopspace{} (\varphi,\varphi_0) \from \loopspace{} \Sc \to \loopspace{} \Sc
    \quad\text{and}\quad
    \loopspace{} (\psi,\psi_0) \from \loopspace{} \Sc \to \loopspace{} \Sc.
  \end{displaymath}
  The elements $\loopspace{} (\varphi,\varphi_0) (\Sloop)$ and
  $\loopspace{} (\psi,\psi_0) (\Sloop)$ of $(\base=\base)$ must be a
  power of $\Sloop$ by the equivalence
  of~\cref{eq:loopspace-circle-Z}. We denote them $\Sloop^k$ and
  $\Sloop^\ell$ respectively. Then the following chain of propositions
  holds:
  \begin{align*}
    \Sloop^{k\ell} &= (\Sloop^k)^\ell\\
    &= \loopspace{} (\varphi,\varphi_0) \left(
      \loopspace{} (\psi,\psi_0) (\Sloop)
    \right)\\
    &= \loopspace{} (\id_\Sc,\pi_{\base}\varphi(\psi_0)\varphi_0) (\Sloop)\\
    &= \inv{\left(\pi_{\base}\varphi(\psi_0)\varphi_0\right)} \Sloop
      \left(\pi_{\base}\varphi(\psi_0)\varphi_0\right)\\
    &= \Sloop
  \end{align*}
  where the last equality exploits commutativity of path composition
  in the loop space $(\base = \base)$. Through the equivalence
  of~\cref{eq:loopspace-circle-Z}, we get that $k\ell=1$ in $\ZZ$,
  from which we get an element of $(k=1)+(k=-1)$. From $k=1$, and
  because
  $\loopspace{} (\varphi,\varphi_0) \jdeq \inv{\varphi_0}
  \varphi(\Sloop) \varphi_0$, one gets an element
  \begin{displaymath}
    b\from \Sloop = \inv{\varphi_0} \varphi(\Sloop)\varphi_0.
  \end{displaymath}
  One can then construct an element $\kappa\from \id_\Sc = \varphi$ by
  $\Sc$-induction by taking $\kappa(\base)$ to be
  $\varphi_0 \from (\base = \varphi(\base))$ and $\ap \kappa(\Sloop)$
  the element $b$ just defined, transported back over the equivalence
  \begin{displaymath}
    (\pathover {\varphi_0} {\id_\Sc(\blank)=\varphi(\blank)} \Sloop {\varphi_0}) \weq
    (\varphi(\Sloop) \varphi_0 \inv \Sloop = \varphi_0)
    \weq (\Sloop = \inv{\varphi_0} \varphi(\Sloop) \varphi_0)
  \end{displaymath}
  By taking $\trunc{\kappa}$, we get an element of
  $\Trunc{\id_\Sc = \varphi}$. Similarly, from $k=-1$, one gets an
  element of $\Trunc{-\id_\Sc =\varphi}$. So in both cases, one gets
  an element of $P(\varphi)$.
\end{proof}

For any type $A$, and an element $a\from A$, let us write $\conncomp A a$
for the connected component of $a$ in $A$. In other words,
\begin{displaymath}
  \conncomp A a \defequi \sum_{x\from A}\Trunc{a=x}.
\end{displaymath}
\cref{lemma:S1-id-neq-minusid} and \cref{prop:S1-eq-either} put
together show that the type $\Sc=\Sc$ has two connected components,
one is the connected component of $\id_\Sc$ and the other is the
connected component of $-\id_\Sc$. In summary, we have shown that
there is an element of the type:
\begin{displaymath}
  (\Sc=\Sc) \weq \conncomp{(\Sc=\Sc)}{\id_\Sc} + \conncomp{(\Sc=\Sc)}{-\id_\Sc}.
\end{displaymath}

In order to prove our goal (cf.~\cref{eq:symm-cricle}), it remains to
exhibit equivalences from $\Sc$ to both
$\conncomp{(\Sc=\Sc)}{\id_\Sc}$ and
$\conncomp{(\Sc=\Sc)}{-\id_\Sc}$. First note that because $\Sc=\Sc$ is
a subtype of $\Sc\to\Sc$, the connected component of some equivalence
$\varphi$ in $\Sc=\Sc$ is equivalent to the connected component of
$\varphi$ seen as a function in $\Sc \to \Sc$. In particular,
\begin{displaymath}
  \conncomp{\left(\Sc=\Sc\right)}{\id_\Sc} \weq \conncomp{\left(\Sc\to\Sc\right)}{\id_\Sc}
  \quad\text{and}\quad
  \conncomp{\left(\Sc=\Sc\right)}{-\id_\Sc} \weq \conncomp{\left(\Sc\to\Sc\right)}{-\id_\Sc}.
\end{displaymath}
Recall that there is an element
\begin{equation}
  \label{eq:S1-loopspace-Z-at-each-x}%
  f\from \prod_{x:\Sc} (\base=\base) \weq (x=x)
\end{equation}
defined by
$\Sc$-induction as the dependent function such that
$f(\base) \jdeq \id_{\base=\base}$ and such that the element
$\ap f (\Sloop) \from (\Sloop\blank\inv\Sloop = \id_{\base=\base})$ is
the reflexivity of $\id_{\base=\base}$ transported along the
commutativity in $\base=\base$. Because $(\base=\base)$ is equivalent
to $\ZZ$ (cf.~\cref{eq:loopspace-circle-Z}), it gives an equivalence
$\varepsilon_x\from (x=x) \weq \ZZ$ for any $x\from\Sc$. We can know
exhibit an equivalence:
\begin{displaymath}
  \begin{tikzcd}
    \left(\Sc \to \Sc\right) \rar["\weq"] & (\sum_{x\from\Sc}x=x)
    \rar["\weq"] & \Sc \times \ZZ
    \\
    \varphi \rar[mapsto] & (\varphi(\base),\ap \varphi (\Sloop))
    \rar[mapsto] & \left(%
      \varphi(\base), \varepsilon_{\varphi(\base)}(\ap\varphi(\Sloop))%
    \right)%
\end{tikzcd}
\end{displaymath}
In particular, one can verify that $\id_\Sc$ is mapped to $(\base,1)$
and $-\id_\Sc$ is mapped to $(\base,-1)$ through this
equivalence. Because $\ZZ$ is a set and $\Sc$ is connected, the
connected components of $\Sc\times\ZZ$ are easy to understand: for
every $x:\Sc$ and $k:\ZZ$, the connected component of $(x,k)$ is
equivalent to the type of all those pairs $(x',k)$ for
$x'\from\Sc$. In particular, every connected component of
$\Sc\times\ZZ$ is equivalent to $\Sc$. In particular, one gets
equivalences:
\begin{displaymath}
  \conncomp{\left(\Sc \to \Sc\right)}{\id_\Sc} \weq \Sc
  \quad\text{and}\quad
  \conncomp{\left(\Sc \to \Sc\right)}{-\id_\Sc} \weq \Sc
\end{displaymath}

Finally, one can compose all the equivalences that we exhibited:
\begin{align*}
  (\Sc=\Sc)
  & \weq \conncomp{\left(\Sc = \Sc\right)}{\id_\Sc}
    + \conncomp{\left(\Sc = \Sc\right)}{-\id_\Sc}
  \\
  & \weq \conncomp{\left(\Sc \to \Sc\right)}{\id_\Sc}
    + \conncomp{\left(\Sc \to \Sc\right)}{-\id_\Sc}
  \\
  & \weq \Sc + \Sc.
\end{align*}

\section{Symmetries of the $2$-sphere}
\label{sec:sphere}

In this section, we will prove that the canonical inclusion:
\begin{equation}
  \label{eq:goal-section-sphere}
  \conncomp{\left(\Sp = \Sp\right)}{\id_\Sp} +
  \conncomp{\left(\Sp = \Sp\right)}{-\id_\Sp}
  \to 
  \left(\Sp = \Sp\right)
\end{equation}
is an equivalence. The equivalence $-\id_\Sp \from \Sp \to \Sp$ is
define by $\Sp$-induction as the function such that
$-\id_\Sp(N) \jdeq S$, and $-\id_\Sp(S) \jdeq N$ and
$\ap{-\id_\Sp}(\mrd x) = \inv{(\mrd x)}$ for all $a\from\Sc$. This
function is indeed an equivalence as it is its own pseudo-inverse.

We will follow more or less the same road map as
in~\cref{sec:circle-case}:
\begin{itemize}
\item first, we will prove that $\id_\Sp$ and $-\id_\Sp$ are not in
  the same connected component,
\item then, we will prove that every equivalence in $\Sp=\Sp$ is
  either in the connected component of $\id_\Sp$ or in the connected
  component of $-\id_\Sp$,
\item finally, we will prove that the connected component of $\id_\Sp$
  and $-\id_\Sp$ are equivalent to each other.
\end{itemize}
Notice that the last step is less ambitious than in the case of $\Sc$,
where the two connected components were proven equivalent to each
other but also each equivalent to $\Sc$ itself. Although we do not
have any counter-argument for it, we do not expect that the connected
components of $\id_\Sp$ and $-\id_\Sp$ are each equivalent to $\Sp$
itself. Indeed, the proof in the case of $\Sc$ relies heavily on two
facts: $\Sc$ is $1$-truncated and $\Sc$ is the classifying type of an
abelian group. In other words, the homotopy structure of $\Sc$ is very
well understood. This is not the case for $\Sp$: for example, it is
certainly not $2$-truncated (\cite{brunerie:thesis}), and it expected
to be provably not $n$-truncated for any $n$.

The main tool for this section is the Hopf family, defined by Brunerie
in~\cite{brunerie:thesis}, to get an analog in HoTT of the Hopf
fibration in topology. First, let us defined for each $x\from\Sc$, an
equivalence $\iota_x\from \Sc=\Sc$ by $\Sc$-induction as the map such
that $\iota_x(\base) \jdeq x$ and $\ap{\iota_x}(\Sloop) = f_x(\Sloop)$
where $f\from \prod_{x\from\Sc} (\base=\base) \weq (x=x)$ is the
dependent function defined
in~\cref{eq:S1-loopspace-Z-at-each-x}. Notice that $\iota_x$ is the
point of $\conncomp{(\Sc=\Sc)}{\id_\Sc}$ that corresponds to $x:\Sc$
under the equivalence $\Sc \weq \conncomp{(\Sc=\Sc)}{\id_\Sc}$
exhibited in~\cref{sec:circle-case}. Now define the type family
$\hopf\from \Sp \to \UU$ by $\Sp$-induction as the family such that
\begin{displaymath}
  \hopf(N) \jdeq \Sc,\quad
  \hopf(S) \jdeq \Sc,\quad\text{and}\quad
  \ap\hopf (\mrd x) = \iota_x\ \text{for all}\ x:\Sc.
\end{displaymath}

\begin{lemma}
  \label{lemma:S2-id-neq-minusid}%
  The proposition $\id_\Sp \neq -\id_\Sp$ holds.
\end{lemma}
\begin{proof}
  Suppose $p:\id_\Sp = -\id_\Sp$ and derive a contradiction. Through
  function extensionality, it produces paths
  \begin{displaymath}
    p(N) \from N = S
    \quad\text{and}\quad
    p(S) \from S = N,
  \end{displaymath}
  and for all $x\from\Sc$ a path over
  $\ap p (\mrd x)\from \pathover {p(N)} T {\mrd x} {p(S)}$ where
  $T\from \Sp \to \UU$ is the type family
  $T(a)\defequi (\id_\Sp(a) = -\id_\Sp(a))$. Because $\Sp$ is simply
  connected and we are targeting the empty type $\varnothing$, which
  is a proposition, we might as well suppose that $p(N)=\mrd \base$
  and $p(S) = \inv{(\mrd \base)}$. Transporting $\ap p(\mrd x)$ over
  these two paths, one gets a path of type
  $\pathover {(\mrd \base)} T {\mrd x} {\inv{(\mrd
      \base)}}$. Transport over $\mrd(x)$ in the type family $T$ is
  easily proven to be equal to the function
  $q \mapsto \inv{\mrd(x)} q \inv{\mrd(x)}$, so that one
  ends up with a path
  \begin{displaymath}
    \pi_x\from \inv{\mrd(x)} \mrd(\base) \inv{\mrd(x)} = \inv{\mrd(\base)}
    \quad
    \text{for all }x\from\Sc
  \end{displaymath}
  In particular, one has
  \begin{displaymath}
    \pi_{\base} \from \inv{\mrd(\base)} \mrd(\base) \inv{\mrd(\base)}
    = \inv{\mrd(\base)}
  \end{displaymath}
  and $\ap {\pi_{\blank}} (\Sloop)$ produces a path
  $\trp [T'] \Sloop (\pi_{\base}) = \pi_{\base}$, where $T'\from\Sc\to\UU$
  is the type family defined by
  \begin{displaymath}
    T'(x) \defequi \left(\inv{\mrd(x)}\mrd(\base)\inv{\mrd(x)}
      = \inv{\mrd(\base)} \right).
  \end{displaymath}
  The type family $T'$ is just a family of path-types with one fixed
  end, so the transport is easily computed:
  \begin{displaymath}
    \trp [T'] \Sloop (\pi_{\base}) = \pi_{\base} \cdot
    \ap{\inv{\mrd(\blank)} \mrd(\base) \inv{\mrd(\blank)}}(\Sloop).
  \end{displaymath}
  Ultimately, one gets a path of type
  \begin{displaymath}
    \ap{\inv{\mrd(\blank)} \mrd(\base) \inv{\mrd(\blank)}}(\Sloop) =
    \refl{\inv{\mrd(\base)} \mrd(\base) \inv{\mrd(\base)}}.
  \end{displaymath}
  However, by path induction on $p\from \base = x$, one can provide an
  element of type
  \begin{displaymath}
    \ap{\inv{\mrd(\blank)} \mrd(\base) \inv{\mrd(\blank)}}(p) =
    \ap{\inv{\mrd(\blank)}}(p) \hcomp \refl{\mrd(\base)}
    \hcomp \ap{\inv{\mrd(\blank)}}(p). 
  \end{displaymath}
  Indeed, for $p\jdeq \refl{\base}$, both sides reduces to
  $\refl{\inv{\mrd(\base)} \mrd(\base) \inv{\mrd(\base)}}$. One can
  apply that in the case $p\jdeq \Sloop$ and
  invoke~\cref{lemma:mustache-lemma} to get an element of type
  \begin{displaymath}
    {\ap{\inv{\mrd(\blank)}}(\Sloop)}^2 = \refl{\inv{\mrd(\base)}}
  \end{displaymath}
  Notice that the term on the left hand-side is equal to
  $\ap{\inv{\blank}}(\ap\mrd (\Sloop^2))$ and the right hand-side is
  equal to $\ap{\inv{\blank}}(\refl{\mrd(\base)})$. Because
  $\inv{\blank}$ is an equivalence, this is equivalently given by an
  element of type
  \begin{displaymath}
    \ap\mrd(\Sloop^2) = \refl{\mrd(\base)}.
  \end{displaymath}
\end{proof}

\section{Symmetries of the $n$-sphere}
\label{sec:higher-sphere}


\bibliographystyle{alpha}
\bibliography{bib}

\end{document}


%%% Local Variables:
%%% mode: latex
%%% TeX-master: t
%%% reftex-default-bibliography: ("bib.bib")
%%% End:
